theories/rules/rules_base.v
@@ -108,7 +108,7 @@ Lemma eliminate_wrong_token {i j E} :
   ▷ (<<j>>) ⊢
   SSWP ExecI @ i ; E {{ _, False }}.
 Proof.
-  iIntros (Hne) ">Htok".
+  iIntros (Hne) "Htok".
   iApply (sswp_lift_atomic_step ExecI) ;[done|].
   iIntros (σ1) "%Hsche Hσ".
   iDestruct "Hσ" as "(Htokown & ? & ? & ? & ? & ? & ? & ?)".
